# Notes on Abstract Algebra 5

# Chapter 2: Groups

### V Normal Subgroups and Cosets

Consider $\phi = sgn:S_3\to \{\pm1\}^{\times}$. (Notation as $x = (1,2,3)$ and $ y = (1,2)$)
$K = \ker \phi = \{1,(1,2,3),(1,3,2)\}\mapsto 1$. $yK = \{(1,2),(1,3),(2,3)\}$.
Question: Can we use the "right coset" of $K = \ker \phi$ to describe fibers of $\phi$?

For $K=\ker \phi$, we have $Ky = yK$. (Reason: $\forall k\in K,\exists k'\in K$ s.t. $yk = k'y$ i.e. $\forall k \in K, yky^{-1}\in K$.)

Definition: We say $N\leq G$ is a normal subgroup ($N\trianglelefteq  G$) if $\forall a \in N \forall g \in G, gag^{-1}\in N$. $gag^{-1}$ are called conjugate of $a$ by $g$.

Proposition: $\forall \phi: G\to G'$ which is a group homomorphism, $\ker\phi$ is a normal subgroup of $G$.

Proof: $\ker \phi\leq G$ is obvious. And $\forall k\in K = \ker \phi, g\in G,\phi(gkg^{-1}) = \phi(g)\phi(k)\phi(g^{-1}) = \phi(g)1_G\phi(g)^{-1} = 1_G$, which implies $gkg^{-1}\in K$.

Some examples of normal subgroups:

- $SL_n(\mathbb R)\trianglelefteq GL_n(\mathbb R)$. ($SL_n(\mathbb R) =\ker \det$).
- $A_n \trianglelefteq S_n(A_n = \ker \text{sgn})$.

Insight: Every kernel is a normal subgroup. What about the inverse "every normal subgroup is a kernel."?

If $G$ is abelian, $H\leq G\Rightarrow H\trianglelefteq G$ since $ghg^{-1} = gg^{-1}h = h\in H$.

A counter example of normal subgroup: $\{1,(12)\}\leq S_3$, but $(1 2 3)(1 2)(123)^{-1} = (2 3)\not \in \{1,(12)\}$.

Another normal subgroup of a group $G$: The center of $G$ (always denoted as $Z$) is defined as $Z(G) = \{z\in G|\forall g\in G,zg = gz\}$ i.e. elements in $Z(G)$ is commutative for every element in $G$. 

Proposition: $Z(G) $ is a normal subgroup of $G$ since $\forall z\in Z(G), \forall g\in G,gzg^{-1} = zgg^{-1}=z\in Z(G)$.

Example: $Z(GL_n(\mathbb R)) = \{\lambda I|\lambda\in \mathbb R^*\}$, $Z(S_3) = \{1\}$. (In fact, $Z(S_n)(n\geq 3) = \{1\}$).

Another way to describe the "commutative level" of two elements $a,b$ is the commutator, defined as $aba^{-1} b^{-1}$. $ab = ba$ if and only if $aba^{-1} b^{-1}=1$.

Remark: The conjugate :$\phi_g: G\to G,\phi(a) = gag^{-1}$ is an automorphism (an isomorphism from $G$ to $G$ self).
